Rename ComIR definitions

ComIR.v
@@ -1,105 +1,105 @@
 From BF Require Import Base Byte VM Token AST.
 
-Inductive ir : Type :=
-  | IRight (n : positive) (i : ir)
-  | ILeft (n : positive) (i : ir)
-  | IAdd (n : byte) (i : ir)
-  | IOutput (i : ir)
-  | IInput (i : ir)
-  | ILoop (body : ir) (i : ir)
-  | IEnd.
+Inductive comir : Type :=
+  | CRight (n : positive) (c : comir)
+  | CLeft (n : positive) (c : comir)
+  | CAdd (n : byte) (c : comir)
+  | COutput (c : comir)
+  | CInput (c : comir)
+  | CLoop (body : comir) (c : comir)
+  | CEnd.
 
-Inductive execute : ir -> vm -> vm -> Prop :=
-  | E_IRight : forall n i v v'',
-      execute i (VM.move_right n v) v'' ->
-      execute (IRight n i) v v''
-  | E_ILeft : forall n i v v' v'',
+Inductive execute : comir -> vm -> vm -> Prop :=
+  | E_CRight : forall n c v v'',
+      execute c (VM.move_right n v) v'' ->
+      execute (CRight n c) v v''
+  | E_CLeft : forall n c v v' v'',
       VM.move_left n (Some v) = Some v' ->
-      execute i v' v'' ->
-      execute (ILeft n i) v v''
-  | E_IAdd : forall n i v v'',
-      execute i (VM.add_cell n v) v'' ->
-      execute (IAdd n i) v v''
-  | E_IOutput : forall i v v'',
-      execute i (VM.output v) v'' ->
-      execute (IOutput i) v v''
-  | E_IInput : forall i v v' v'',
+      execute c v' v'' ->
+      execute (CLeft n c) v v''
+  | E_CAdd : forall n c v v'',
+      execute c (VM.add_cell n v) v'' ->
+      execute (CAdd n c) v v''
+  | E_COutput : forall c v v'',
+      execute c (VM.output v) v'' ->
+      execute (COutput c) v v''
+  | E_CInput : forall c v v' v'',
       VM.input v = Some v' ->
-      execute i v' v'' ->
-      execute (IInput i) v v''
-  | E_ILoop : forall body i v v' v'',
+      execute c v' v'' ->
+      execute (CInput c) v v''
+  | E_CLoop : forall body c v v' v'',
       VM.get_cell v =? #00 = false ->
       execute body v v' ->
-      execute (ILoop body i) v' v'' ->
-      execute (ILoop body i) v v''
-  | E_ILoop_0 : forall body i v v',
+      execute (CLoop body c) v' v'' ->
+      execute (CLoop body c) v v''
+  | E_CLoop_0 : forall body c v v',
       VM.get_cell v =? #00 = true ->
-      execute i v v' ->
-      execute (ILoop body i) v v'
-  | E_IEnd : forall v,
-      execute IEnd v v.
+      execute c v v' ->
+      execute (CLoop body c) v v'
+  | E_CEnd : forall v,
+      execute CEnd v v.
 
-Definition equiv (i1 i2 : ir) : Prop := forall v v',
+Definition equiv (i1 i2 : comir) : Prop := forall v v',
   execute i1 v v' <-> execute i2 v v'.
 
-Definition transform_sound (trans : ir -> ir) : Prop := forall i,
-  equiv i (trans i).
+Definition transform_sound (trans : comir -> comir) : Prop := forall c,
+  equiv c (trans c).
 
-Fixpoint cons_right (n : positive) (i : ir) : ir :=
-  match i with
-  | IRight m i' => IRight (n + m) i'
-  | ILeft m i' => match n ?= m with
-                  | Eq => i'
-                  | Lt => ILeft (m - n) i'
-                  | Gt => cons_right (n - m) i'
+Fixpoint cons_right (n : positive) (c : comir) : comir :=
+  match c with
+  | CRight m c' => CRight (n + m) c'
+  | CLeft m c' => match n ?= m with
+                  | Eq => c'
+                  | Lt => CLeft (m - n) c'
+                  | Gt => cons_right (n - m) c'
                   end
-  | _ => IRight n i
+  | _ => CRight n c
   end%positive.
 
-Definition cons_left (n : positive) (i : ir) : ir :=
-  match i with
-  | ILeft m i' => ILeft (n + m) i'
-  | _ => ILeft n i
+Definition cons_left (n : positive) (c : comir) : comir :=
+  match c with
+  | CLeft m c' => CLeft (n + m) c'
+  | _ => CLeft n c
   end.
 
-Definition cons_add (n : byte) (i : ir) : ir :=
-  match i with
-  | IAdd m i' => IAdd (n + m) i'
-  | _ => IAdd n i
+Definition cons_add (n : byte) (c : comir) : comir :=
+  match c with
+  | CAdd m c' => CAdd (n + m) c'
+  | _ => CAdd n c
   end.
 
-Fixpoint lower_ast (a : ast) : ir :=
+Fixpoint lower_ast (a : ast) : comir :=
   match a with
-  | ARight a' => IRight 1 (lower_ast a')
-  | ALeft a' => ILeft 1 (lower_ast a')
-  | AInc a' => IAdd #01 (lower_ast a')
-  | ADec a' => IAdd #ff (lower_ast a')
-  | AOutput a' => IOutput (lower_ast a')
-  | AInput a' => IInput (lower_ast a')
-  | ALoop body a' => ILoop (lower_ast body) (lower_ast a')
-  | AEnd => IEnd
+  | ARight a' => CRight 1 (lower_ast a')
+  | ALeft a' => CLeft 1 (lower_ast a')
+  | AInc a' => CAdd #01 (lower_ast a')
+  | ADec a' => CAdd #ff (lower_ast a')
+  | AOutput a' => COutput (lower_ast a')
+  | AInput a' => CInput (lower_ast a')
+  | ALoop body a' => CLoop (lower_ast body) (lower_ast a')
+  | AEnd => CEnd
   end.
 
-Fixpoint raise_ast (i : ir) : ast :=
-  match i with
-  | IRight n i' => AST.cons_right n (raise_ast i')
-  | ILeft n i' => AST.cons_left n (raise_ast i')
-  | IAdd n i' => AST.cons_add n (raise_ast i')
-  | IOutput i' => AOutput (raise_ast i')
-  | IInput i' => AInput (raise_ast i')
-  | ILoop body i' => ALoop (raise_ast body) (raise_ast i')
-  | IEnd => AEnd
+Fixpoint raise_ast (c : comir) : ast :=
+  match c with
+  | CRight n c' => AST.cons_right n (raise_ast c')
+  | CLeft n c' => AST.cons_left n (raise_ast c')
+  | CAdd n c' => AST.cons_add n (raise_ast c')
+  | COutput c' => AOutput (raise_ast c')
+  | CInput c' => AInput (raise_ast c')
+  | CLoop body c' => ALoop (raise_ast body) (raise_ast c')
+  | CEnd => AEnd
   end.
 
-Fixpoint combine (i : ir) : ir :=
-  match i with
-  | IRight n i' => cons_right n (combine i')
-  | ILeft n i' => cons_left n (combine i')
-  | IAdd n i' => cons_add n (combine i')
-  | IOutput i' => IOutput (combine i')
-  | IInput i' => IInput (combine i')
-  | ILoop body i' => ILoop (combine body) (combine i')
-  | IEnd => IEnd
+Fixpoint combine (c : comir) : comir :=
+  match c with
+  | CRight n c' => cons_right n (combine c')
+  | CLeft n c' => cons_left n (combine c')
+  | CAdd n c' => cons_add n (combine c')
+  | COutput c' => COutput (combine c')
+  | CInput c' => CInput (combine c')
+  | CLoop body c' => CLoop (combine body) (combine c')
+  | CEnd => CEnd
   end.
 
 Example test_execute : forall a,
@@ -107,14 +107,14 @@ Example test_execute : forall a,
   execute (lower_ast a) (VM.make [#02]) (VM [] #07 [] [#07] []).
 Proof.
   intros. inversion H; subst; clear H.
-  repeat (apply E_IRight
-       || (eapply E_ILeft; [reflexivity |])
-       || apply E_IAdd
-       || apply E_IOutput
-       || (eapply E_IInput; [reflexivity |])
-       || (eapply E_ILoop; [reflexivity | |])
-       || (eapply E_ILoop_0; [reflexivity |])
-       || apply E_IEnd).
+  repeat (apply E_CRight
+       || (eapply E_CLeft; [reflexivity |])
+       || apply E_CAdd
+       || apply E_COutput
+       || (eapply E_CInput; [reflexivity |])
+       || (eapply E_CLoop; [reflexivity | |])
+       || (eapply E_CLoop_0; [reflexivity |])
+       || apply E_CEnd).
   (* TODO: Normalize right tape and bytes *)
 Admitted.
 
@@ -147,62 +147,62 @@ Ltac destruct_compare n m :=
   | rewrite Pos.compare_lt_iff in Hcomp
   | rewrite Pos.compare_gt_iff in Hcomp].
 
-Theorem cons_right_correct : forall i n v v',
-  execute (cons_right n i) v v' <-> execute (IRight n i) v v'.
+Theorem cons_right_correct : forall c n v v',
+  execute (cons_right n c) v v' <-> execute (CRight n c) v v'.
 Proof.
   split;
   generalize dependent v'; generalize dependent v; generalize dependent n.
-  - induction i; cbn; intros; try assumption.
+  - induction c; cbn; intros; try assumption.
     + inversion H; subst.
-      apply E_IRight, E_IRight. rewrite VM.move_right_add. assumption.
+      apply E_CRight, E_CRight. rewrite VM.move_right_add. assumption.
     + destruct_compare n0 n.
-      * eapply E_IRight, E_ILeft. apply VM.move_right_left_refl.
+      * eapply E_CRight, E_CLeft. apply VM.move_right_left_refl.
         admit. assumption.
       * inversion H; subst.
-        eapply E_IRight, E_ILeft. rewrite VM.move_right_left_lt.
+        eapply E_CRight, E_CLeft. rewrite VM.move_right_left_lt.
         eassumption. admit. apply Hcomp. assumption.
-      * apply IHi in H. inversion H; subst.
-        eapply E_IRight, E_ILeft. apply VM.move_right_left_gt.
+      * apply IHc in H. inversion H; subst.
+        eapply E_CRight, E_CLeft. apply VM.move_right_left_gt.
         admit. apply Hcomp. assumption.
-  - induction i; cbn; intros; try assumption;
+  - induction c; cbn; intros; try assumption;
     inversion H; inversion H4; subst.
     + rewrite VM.move_right_add in H9.
-      apply E_IRight. assumption.
+      apply E_CRight. assumption.
     + destruct_compare n0 n.
       * rewrite VM.move_right_left_refl in H7. inversion H7; subst.
         assumption. admit.
       * rewrite VM.move_right_left_lt in H7.
-        eapply E_ILeft. eassumption. assumption. admit. apply Hcomp.
+        eapply E_CLeft. eassumption. assumption. admit. apply Hcomp.
       * rewrite VM.move_right_left_gt in H7. inversion H7; subst.
-        apply IHi. apply E_IRight. assumption. admit. assumption.
+        apply IHc. apply E_CRight. assumption. admit. assumption.
 Admitted.
 
-Theorem cons_left_correct : forall i n v v',
-  execute (cons_left n i) v v' <-> execute (ILeft n i) v v'.
+Theorem cons_left_correct : forall c n v v',
+  execute (cons_left n c) v v' <-> execute (CLeft n c) v v'.
 Proof.
   split;
   generalize dependent v'; generalize dependent v; generalize dependent n.
-  - destruct i; cbn; intros; try assumption.
+  - destruct c; cbn; intros; try assumption.
     inversion H; subst.
     rewrite Pos.add_comm, <- VM.move_left_add in H2.
     apply VM.move_left_split in H2 as [v'1 []].
-    eapply E_ILeft, E_ILeft; eassumption.
-  - destruct i; cbn; intros; try assumption.
+    eapply E_CLeft, E_CLeft; eassumption.
+  - destruct c; cbn; intros; try assumption.
     inversion H; inversion H5; subst.
-    rewrite Pos.add_comm. eapply E_ILeft. rewrite <- VM.move_left_add.
+    rewrite Pos.add_comm. eapply E_CLeft. rewrite <- VM.move_left_add.
     rewrite H2. eassumption. assumption.
 Qed.
 
-Theorem cons_add_correct : forall i n v v',
-  execute (cons_add n i) v v' <-> execute (IAdd n i) v v'.
+Theorem cons_add_correct : forall c n v v',
+  execute (cons_add n c) v v' <-> execute (CAdd n c) v v'.
 Proof.
   split.
-  - destruct i; cbn; intros; try assumption.
+  - destruct c; cbn; intros; try assumption.
     inversion H; subst.
-    apply E_IAdd, E_IAdd. rewrite VM.add_add. assumption.
-  - destruct i; cbn; intros; try assumption.
+    apply E_CAdd, E_CAdd. rewrite VM.add_add. assumption.
+  - destruct c; cbn; intros; try assumption.
     inversion H; inversion H4; subst.
-    apply E_IAdd. rewrite <- VM.add_add. assumption.
+    apply E_CAdd. rewrite <- VM.add_add. assumption.
 Qed.
 
 Theorem combine_sound :
@@ -212,23 +212,23 @@ Proof.
   split.
   - intros. induction H; cbn;
     try (econstructor; eassumption).
-    + rewrite cons_right_correct. apply E_IRight. assumption.
-    + rewrite cons_left_correct. eapply E_ILeft; eassumption.
-    + rewrite cons_add_correct. apply E_IAdd. assumption.
+    + rewrite cons_right_correct. apply E_CRight. assumption.
+    + rewrite cons_left_correct. eapply E_CLeft; eassumption.
+    + rewrite cons_add_correct. apply E_CAdd. assumption.
   - generalize dependent v'; generalize dependent v.
-    induction i; intros; cbn in *.
+    induction c; intros; cbn in *.
     + rewrite cons_right_correct in H. inversion H; subst.
-      apply E_IRight, IHi. assumption.
+      apply E_CRight, IHc. assumption.
     + rewrite cons_left_correct in H. inversion H; subst.
-      eapply E_ILeft. eassumption. apply IHi. assumption.
+      eapply E_CLeft. eassumption. apply IHc. assumption.
     + rewrite cons_add_correct in H. inversion H; subst.
-      apply E_IAdd, IHi. assumption.
-    + inversion H; subst. constructor. apply IHi. assumption.
-    + inversion H; subst. econstructor. eassumption. apply IHi. assumption.
+      apply E_CAdd, IHc. assumption.
+    + inversion H; subst. constructor. apply IHc. assumption.
+    + inversion H; subst. econstructor. eassumption. apply IHc. assumption.
     + dependent induction H.
-      * eapply E_ILoop. assumption. apply IHi1. eassumption.
+      * eapply E_CLoop. assumption. apply IHc1. eassumption.
         apply IHexecute2; try assumption. reflexivity.
-      * apply E_ILoop_0, IHi2; assumption.
+      * apply E_CLoop_0, IHc2; assumption.
     + assumption.
 Qed.
 
