README.md
@@ -2,6 +2,13 @@
 
 A formally verified Brainfuck compiler in Coq using Hoare logic.
 
+## Stages
+
+- [`Token`](Token.v): Flat lexical tokens
+- [`AST`](AST.v): Inductive loops
+- [`ComIR`](ComIR.v): Combined sequences of `>`, `<`, `+`, and `-`
+- RelIR: Relative-positioned cell offsets
+
 ## Installation
 
 bfcoq requires CompCert for its `byte` type. [Using opam](https://coq.inria.fr/opam-using.html),
